wip on #11

pulse/src/checker/Pulse.Steel.Wrapper.Typing.fst
@@ -44,3 +44,5 @@ let stt_ghost_admit_typing _ _ _ = admit ()
 let rewrite_typing _ _ _ = admit ()
 let with_local_typing _ _ _ _ _ _ _ = admit ()
 let with_localarray_typing _ _ _ _ _ _ _ _ = admit ()
+
+let squash_non_informative_witness_typing _ = admit ()
